Strata/Languages/Core/StatementSemanticsProps.lean
@@ -849,7 +849,7 @@ theorem updatedStateComm'
 theorem updatedStatesComm
   {P : PureExpr} {σ : SemanticStore P}
   {kvs kvs' : List (P.Ident × P.Expr)} :
-  kvs.unzip.1.Disjoint kvs'.unzip.1 →
+  kvs.unzip.1.Disj kvs'.unzip.1 →
   updatedStates' (updatedStates' σ kvs) kvs' =
   updatedStates' (updatedStates' σ kvs') kvs := by
   intros Hnd
@@ -861,14 +861,14 @@ theorem updatedStatesComm
     rw [updatedStateComm]
     rw [updatedStateComm']
     . simp at Hnd
-      have Hnd' := List.Disjoint.symm Hnd
+      have Hnd' := List.Disj.symm Hnd
       apply List.Disjoint_cons_head
-      apply List.Disjoint.mono_right _ Hnd'
+      apply List.Disj.mono_right _ Hnd'
       simp_all
     . intros Hin
-      simp_all [List.Disjoint]
+      simp_all [List.Disj]
     . simp at *
-      refine List.Disjoint.mono_right ?_ Hnd
+      refine List.Disj.mono_right ?_ Hnd
       simp_all
 
 theorem UpdateStateSomeMonotone
@@ -1208,7 +1208,7 @@ specialize Hnin k1
 simp_all
 
 theorem substStoresUpdatesInv :
-ks.Disjoint substs.unzip.2 →
+ks.Disj substs.unzip.2 →
 substStores σ σ' substs →
 UpdateStates σ' ks vs σ'' →
 substStores σ σ'' substs := by
@@ -1220,7 +1220,7 @@ case update_none =>
   exact Hsubst k1 k2 Hin
 case update_some σ x v σ' xs vs σ₁ Hup Hinits ih =>
   have Hnin : ¬ x ∈ substs.unzip.2 := by
-    simp [List.Disjoint] at Hnin
+    simp [List.Disj] at Hnin
     intros Hin
     have Hprod := List.mem_zip_2 (l₁:=substs.unzip.fst) (by simp) Hin
     rw [List.zip_unzip] at Hprod
@@ -1230,11 +1230,11 @@ case update_some σ x v σ' xs vs σ₁ Hup Hinits ih =>
     contradiction
   have HH := substStoresUpdateInv (σ:=σ) Hnin Hsubst Hup
   apply ih HH
-  simp [List.Disjoint] at *
+  simp [List.Disj] at *
   simp_all
 
 theorem substStoresUpdatesInv' :
-ks.Disjoint substs.unzip.1 →
+ks.Disj substs.unzip.1 →
 substStores σ σ' substs →
 UpdateStates σ ks vs σ'' →
 substStores σ'' σ' substs := by
@@ -1629,7 +1629,7 @@ theorem InitStateDefMonotone'
     exact Hdef Hv'
 
 theorem InitStatesDefMonotone' :
-  vs.Disjoint vs' →
+  vs.Disj vs' →
   isDefined σ' vs →
   InitStates σ vs' es' σ' →
   isDefined σ vs := by
@@ -1643,12 +1643,12 @@ theorem InitStatesDefMonotone' :
     apply Hdisj Hin
     exact List.mem_cons_self
   . apply ih
-    . apply List.Disjoint.mono_right _ Hdisj
+    . apply List.Disj.mono_right _ Hdisj
       exact List.sublist_cons_self x xs'
     . assumption
 
 theorem InitVarsDefMonotone' :
-  vs.Disjoint vs' →
+  vs.Disj vs' →
   isDefined σ' vs →
   InitVars σ vs' σ' →
   isDefined σ vs := by
@@ -1659,7 +1659,7 @@ theorem InitVarsDefMonotone' :
   exact InitStatesDefMonotone' Hdisj Hdef Hinit
 
 -- theorem InitVarsNotDefMonotone' :
---   vs.Disjoint vs' →
+--   vs.Disj vs' →
 --   isDefined σ' vs →
 --   InitVars σ vs' σ' →
 --   isNotDefined σ vs := by
@@ -1842,7 +1842,7 @@ theorem InvStoresUpdatedStateDisjRightMono :
       exact H
 
 theorem InvStoresUpdatedStatesDisjRightMono :
-  ks.Disjoint ks' →
+  ks.Disj ks' →
   invStores σ σ' ks →
   ks'.length = vs'.length →
   invStores σ (updatedStates σ' ks' vs') ks := by
@@ -1878,7 +1878,7 @@ theorem InvStoresUpdatedStateDisjLeftMono :
   exact InvStoresUpdatedStateDisjRightMono Hnin Hinv'
 
 theorem InvStoresUpdatedStatesDisjLeftMono :
-  ks.Disjoint ks' →
+  ks.Disj ks' →
   invStores σ σ' ks →
   ks'.length = vs'.length →
   invStores (updatedStates σ ks' vs') σ' ks := by
@@ -1901,7 +1901,7 @@ theorem InvStoresExceptApp :
   invStoresExcept σ σ' (ks ++ ks') := by
   intros Hinv x Hdisj
   apply Hinv
-  exact List.DisjointAppRight' Hdisj
+  exact List.DisjAppRight' Hdisj
 
 theorem InvStoresExceptUpdated :
   invStoresExcept σ σ' ks →
@@ -1911,9 +1911,9 @@ theorem InvStoresExceptUpdated :
   simp [invStoresExcept] at *
   intros vsInv Hdisj
   refine InvStoresUpdatedStatesDisjLeftMono ?_ ?_ Hlen
-  exact List.DisjointAppLeft' Hdisj
+  exact List.DisjAppLeft' Hdisj
   apply Hinv
-  exact List.DisjointAppRight' Hdisj
+  exact List.DisjAppRight' Hdisj
 
 theorem UpdatedStatesInSame :
   k ∈ ks' →
@@ -2044,11 +2044,11 @@ theorem InvStoresExceptInitVars :
 
 theorem InvStoresExceptInvStores :
   invStoresExcept σ σ' ks →
-  List.Disjoint ks ks' →
+  List.Disj ks ks' →
   invStores σ σ' ks' := by
   intros Hinv Hdis k1 k2 Hin
   apply Hinv ks'
-  exact List.Disjoint.symm Hdis
+  exact List.Disj.symm Hdis
   assumption
 
 
